coq/src/auction.v
@@ -488,8 +488,10 @@ Definition auction_item
   : public_byte_seq :=
   seq_new_ (@repr WORDSIZE8 0) (usize 0).
 
-Definition auction_test_init (item_57 : public_byte_seq) : bool :=
-  let time_58 : int64 := @repr WORDSIZE64 1 in 
+Definition auction_test_init
+  (item_57 : public_byte_seq)
+  (time_58 : int64) `{(item_57) = (auction_item (repr 0) (repr 1) (repr 2))} `{(time_58) = (repr 1)}
+  : bool :=
   (fresh_state ((item_57)) (time_58)) =.? (State ((
         NotSoldYet,
         @repr WORDSIZE64 0,
@@ -500,11 +502,13 @@ Definition auction_test_init (item_57 : public_byte_seq) : bool :=
             seq_new_ (@repr WORDSIZE8 0) (usize 0)
           ))
       ))).
-Theorem ensures_auction_test_init : forall result (item : public_byte_seq),
 
-auction_test_init item = result ->
-((result) = (true)).
-Proof. Admitted.
+Theorem ensures_auction_test_init : forall result (item_57 : public_byte_seq) (time_58 : int64),
+forall {H_0 : (item_57) = (auction_item (repr 0) (repr 1) (repr 2))},
+forall {H_1 : (time_58) = (repr 1)},
+@auction_test_init item_57 time_58 H_0 H_1= result ->
+(result) = (true).
+Proof. now (intros ; subst). Qed.
 
 Definition verify_bid
   (item_59 : public_byte_seq)
@@ -588,7 +592,7 @@ Definition new_account
 
 Definition test_auction_bid_and_finalize
   (item_79 : public_byte_seq)
-  (time_80 : int64) `{(forall i, (((repr 0) <= (item)) /\ ((i) < (len (TODOUnaryitem)))) -> ((get (TODOFinalitem) (i)) = (Some (repr 0))))}
+  (time_80 : int64) `{(item_79) = (auction_item (repr 0) (repr 1) (repr 5))} `{(time_80) = (repr 1)}
   : bool :=
   let amount_81 : int64 := @repr WORDSIZE64 100 in 
   let winning_amount_82 : int64 := @repr WORDSIZE64 300 in 
@@ -655,9 +659,14 @@ Definition test_auction_bid_and_finalize
     | Ok _ => false
     end in 
   (((((((result_0_91) && (result_1_95)) && (result_2_101)) && (result_3_107)) && (result_4_115)) && (result_5_118)) && (result_6_121)) && (result_7_126).
-Theorem ensures_test_auction_bid_and_finalize : forall result (item : public_byte_seq) (time : int64),
-(forall i, (((repr 0) <= (item)) /\ ((i) < (len (TODOUnaryitem)))) -> ((get (TODOFinalitem) (i)) = (Some (repr 0))))->
-test_auction_bid_and_finalize item time = result ->
-((TODOModelresult) = (((a), (b)))).
-Proof. Admitted.
 
+Theorem ensures_test_auction_bid_and_finalize : forall result (item_79 : public_byte_seq) (time_80 : int64),
+forall {H_0 : (item_79) = (auction_item (repr 0) (repr 1) (repr 5))},
+forall {H_1 : (time_80) = (repr 1)},
+@test_auction_bid_and_finalize item_79 time_80 H_0 H_1= result ->
+(result) = (true).
+Proof.
+  intros.
+  subst.
+  reflexivity.
+Qed.
